Add more basis module stubs, and update helloProg
The aim is to get ioProg to depend on these modules, so have moved
bits of its prefix into the modules.

basis/basisFunctionsLib.sml
@@ -1,4 +1,4 @@
-structure basisFunctionsLib :> basisFunctionsLib = 
+structure basisFunctionsLib :> basisFunctionsLib =
 struct
 
 open preamble
@@ -50,5 +50,20 @@ fun prove_ref_spec op_name =
   fs [cf_ref_def, cf_deref_def, cf_assign_def] \\ irule local_elim \\
   reduce_tac \\ fs [app_ref_def, app_deref_def, app_assign_def] \\
   xsimpl \\ fs [UNIT_TYPE_def]
+
+fun derive_eval_thm v_name e = let
+  val th = get_ml_prog_state () |> get_thm
+  val th = MATCH_MP ml_progTheory.ML_code_NONE_Dlet_var th
+           handle HOL_ERR _ =>
+           MATCH_MP ml_progTheory.ML_code_SOME_Dlet_var th
+  val goal = th |> SPEC e |> SPEC_ALL |> concl |> dest_imp |> fst
+  val lemma = goal
+    |> (NCONV 50 (SIMP_CONV (srw_ss()) [Once bigStepTheory.evaluate_cases,
+            PULL_EXISTS,do_app_def,store_alloc_def,LET_THM]) THENC EVAL)
+  val v_thm = prove(mk_imp(lemma |> concl |> rand,goal),fs [lemma])
+                 |> GEN_ALL |> SIMP_RULE std_ss [] |> SPEC_ALL
+  val v_tm = v_thm |> concl |> rand |> rand |> rand
+  val v_def = define_abbrev true v_name v_tm
+  in v_thm |> REWRITE_RULE [GSYM v_def] end
 
 end
