characteristic/examples/helloProgScript.sml
@@ -2,93 +2,13 @@ open preamble
      semanticPrimitivesTheory
      ml_translatorTheory ml_translatorLib ml_progLib
      cfHeapsTheory cfTheory cfTacticsBaseLib cfTacticsLib
-     mlw8arrayProgTheory basisFunctionsLib
+     mlcharioProgTheory basisFunctionsLib
 
 val _ = new_theory "helloProg"
 
-val _ = translation_extends"mlw8arrayProg";
+val _ = translation_extends"mlcharioProg";
 
 fun basis_st () = get_ml_prog_state ()
-
-(* TODO: these modules should be inherited rather than re-verified here *)
-
-(* Word8Array module -- CF verified *)
-
-
-(* CharIO -- CF verified *)
-
-val _ = ml_prog_update (open_module "CharIO");
-
-fun derive_eval_thm v_name e = let
-  val th = get_ml_prog_state () |> get_thm
-  val th = MATCH_MP ml_progTheory.ML_code_NONE_Dlet_var th
-           handle HOL_ERR _ =>
-           MATCH_MP ml_progTheory.ML_code_SOME_Dlet_var th
-  val goal = th |> SPEC e |> SPEC_ALL |> concl |> dest_imp |> fst
-  val lemma = goal
-    |> (NCONV 50 (SIMP_CONV (srw_ss()) [Once bigStepTheory.evaluate_cases,
-            PULL_EXISTS,do_app_def,store_alloc_def,LET_THM]) THENC EVAL)
-  val v_thm = prove(mk_imp(lemma |> concl |> rand,goal),fs [lemma])
-                 |> GEN_ALL |> SIMP_RULE std_ss [] |> SPEC_ALL
-  val v_tm = v_thm |> concl |> rand |> rand |> rand
-  val v_def = define_abbrev true v_name v_tm
-  in v_thm |> REWRITE_RULE [GSYM v_def] end
-
-val e = ``(App Aw8alloc [Lit (IntLit 1); Lit (Word8 0w)])``
-
-val _ = ml_prog_update (add_Dlet (derive_eval_thm "write_loc" e) "write" [])
-
-val Apps_def = tDefine "Apps" `
-  (Apps [x;y] = App Opapp [x;y]) /\
-  (Apps [] = ARB) /\
-  (Apps xs = App Opapp [Apps (FRONT xs); LAST xs])`
-  (WF_REL_TAC `measure LENGTH` \\ fs [LENGTH_FRONT]);
-
-val LetApps_def = Define `
-  LetApps n f args = Let (SOME n) (Apps (Var f::args))`;
-
-val e =
-  ``Let (SOME "c") (Apps [Var (Long "Word8Array" "update"); Var (Short "write");  Lit (IntLit 0); Var (Short "c")])
-     (Let (SOME "_") (App (FFI "write") [Var (Short "write")])
-        (Var (Short "c")))``
-  |> EVAL |> concl |> rand
-
-val _ = ml_prog_update (add_Dlet_Fun ``"write"`` ``"c"`` e "write_v")
-
-val _ = ml_prog_update (close_module NONE);
-
-val stdout_fun_def = Define `
-  stdout_fun = (\_ bytes s. case (bytes,s) of (* write *)
-                    | ([w],Str output) => SOME ([w],Str (output ++ [CHR (w2n w)]))
-                    | _ => NONE)`
-
-val STDOUT_def = Define `
-  STDOUT output = IO (Str output) stdout_fun ["write"]`
-
-val CHAR_IO_def = Define `
-  CHAR_IO = SEP_EXISTS w. W8ARRAY write_loc [w]`;
-
-val write_spec = Q.store_thm ("write_spec",
-  `!a av n nv v.
-     WORD (c:word8) cv ==>
-     app (p:'ffi ffi_proj) ^(fetch_v "CharIO.write" (basis_st()))
-       [cv]
-       (CHAR_IO * STDOUT output)
-       (POSTv uv. cond (UNIT_TYPE () uv) * CHAR_IO * STDOUT (output ++ [CHR (w2n c)]))`,
-  xcf "CharIO.write" (basis_st())
-  \\ fs [CHAR_IO_def] \\ xpull
-  \\ xlet `POSTv zv. STDOUT output * W8ARRAY write_loc [c] *
-                     & (UNIT_TYPE () zv)`
-  THEN1
-   (xapp \\ xsimpl \\ fs [CHAR_IO_def,EVAL ``write_loc``]
-    \\ instantiate \\ xsimpl \\ EVAL_TAC \\ fs [])
-  \\ xlet `POSTv _. STDOUT (output ++ [CHR (w2n c)]) * W8ARRAY write_loc [c]`
-  THEN1
-   (xffi
-    \\ fs [EVAL ``write_loc``, STDOUT_def]
-    \\ `MEM "write" ["write"]` by EVAL_TAC \\ instantiate \\ xsimpl
-    \\ EVAL_TAC \\ fs [ORD_BOUND, CHR_ORD])
-  \\ xret \\ xsimpl);
 
 val e =
   ``LetApps "_" (Long "CharIO" "write") [Lit (Word8 (n2w (ORD #"H")))]
@@ -101,14 +21,14 @@ val main_spec = Q.store_thm ("main",
   `!cv input output.
       app (p:'ffi ffi_proj) ^(fetch_v "main" (basis_st()))
         [cv]
-        (CHAR_IO * STDOUT "")
-        (POSTv uv. CHAR_IO * STDOUT "Hi")`,
+        (STDOUT [])
+        (POSTv uv. STDOUT (MAP (n2w o ORD) "Hi"))`,
   xcf "main" (basis_st())
-  \\ xlet `POSTv v. CHAR_IO * STDOUT "H"` THEN1
-   (xapp \\ qexists_tac `emp` \\ qexists_tac `""` \\ qexists_tac `n2w (ORD #"H")`
+  \\ xlet `POSTv v. STDOUT [n2w(ORD #"H")]` THEN1
+   (xapp \\ qexists_tac `emp` \\ qexists_tac `[]` \\ qexists_tac `n2w (ORD #"H")`
     \\ xsimpl)
-  \\ xlet `POSTv v. CHAR_IO * STDOUT "Hi"` THEN1
-   (xapp \\ qexists_tac `emp` \\ qexists_tac `"H"` \\ qexists_tac `n2w (ORD #"i")`
+  \\ xlet `POSTv v. STDOUT (MAP (n2w o ORD) "Hi")` THEN1
+   (xapp \\ qexists_tac `emp` \\ qexists_tac `[n2w(ORD #"H")]` \\ qexists_tac `n2w (ORD #"i")`
     \\ xsimpl)
   \\ xvar \\ fs [] \\ xsimpl);
 
