basis/mlcharioProgScript.sml
@@ -1,0 +1,183 @@
+open preamble
+     ml_translatorLib ml_progLib
+     cfTheory cfHeapsTheory cfTacticsLib cfTacticsBaseLib basisFunctionsLib
+     mlw8arrayProgTheory
+
+val _ = new_theory "mlcharioProg";
+
+val _ = translation_extends "mlw8arrayProg";
+
+(* TODO: where should these be defined? *)
+
+val Apps_def = tDefine "Apps" `
+  (Apps [x;y] = App Opapp [x;y]) /\
+  (Apps [] = ARB) /\
+  (Apps xs = App Opapp [Apps (FRONT xs); LAST xs])`
+  (WF_REL_TAC `measure LENGTH` \\ fs [LENGTH_FRONT]);
+
+val LetApps_def = Define `
+  LetApps n f args = Let (SOME n) (Apps (Var f::args))`;
+
+(* -- *)
+
+(* CharIO -- CF verified *)
+
+val _ = ml_prog_update (open_module "CharIO");
+
+(* TODO: do these occur more naturally somewhere else in the basis ? *)
+val _ = trans "bool_of_byte" `\(w:word8). w <> 0w`
+val _ = trans "char_of_byte" `\(w:word8). CHR (w2n w)`
+
+val chario_char_of_byte_side = Q.store_thm("chario_char_of_byte_side",
+  `chario_char_of_byte_side w`,
+  metis_tac [fetch"-" "chario_char_of_byte_side_def",w2n_lt,EVAL ``dimword(:8)``]);
+(* -- *)
+
+val e = ``(App Aw8alloc [Lit (IntLit 2); Lit (Word8 0w)])``
+
+val _ = ml_prog_update (add_Dlet (derive_eval_thm "read_state_loc" e) "read_state" [])
+
+val e = ``(App Aw8alloc [Lit (IntLit 1); Lit (Word8 0w)])``
+
+val _ = ml_prog_update (add_Dlet (derive_eval_thm "write_state_loc" e) "write_state" [])
+
+val e =
+  ``Let NONE (App (FFI "getChar") [Var (Short "read_state")])
+     (LetApps "c" (Long "Word8Array" "sub") [Var (Short "read_state");  Lit (IntLit 0)]
+       (Apps [Var (Short "char_of_byte"); Var (Short "c")]))``
+  |> EVAL |> concl |> rand
+
+val _ = ml_prog_update (add_Dlet_Fun ``"read"`` ``"u"`` e "read_v")
+
+val e =
+  ``LetApps "f" (Long "Word8Array" "sub") [Var (Short "read_state"); Lit (IntLit 1)]
+      (Apps [Var (Short "bool_of_byte"); Var (Short "f")])``
+  |> EVAL |> concl |> rand
+
+val _ = ml_prog_update (add_Dlet_Fun ``"read_failed"`` ``"u"`` e "read_failed_v")
+
+val e =
+  ``Let (SOME "c") (Apps [Var (Long "Word8Array" "update");
+                          Var (Short "write_state");
+                          Lit (IntLit 0); Var (Short "c")])
+      (Let NONE (App (FFI "putChar") [Var (Short "write_state")]) (Var (Short "c")))``
+  |> EVAL |> concl |> rand
+
+val _ = ml_prog_update (add_Dlet_Fun ``"write"`` ``"c"`` e "write_v")
+
+val _ = ml_prog_update (close_module NONE);
+
+val stdin_fun_def = Define `
+  stdin_fun = (\i bytes s. case (bytes,s) of
+                    | ([b;f],Str input) =>
+                         if i = "getChar" then (* read *)
+                           if input = "" then
+                             SOME ([b;1w],Str input)
+                           else (* i = "putChar" *)
+                             SOME ([n2w (ORD (HD input)); 0w],Str (TL input))
+                         else NONE
+                    | _ => NONE)`
+
+val stdout_fun_def = Define `
+  stdout_fun = (\_ bytes s. case (bytes,s) of (* write *)
+                    | ([w],Str output) => SOME ([w],Str (output ++ [CHR (w2n w)]))
+                    | _ => NONE)`
+
+val STDIN_def = Define `
+  STDIN input read_failed =
+    IO (Str input) stdin_fun ["getChar"] *
+    SEP_EXISTS w. W8ARRAY read_state_loc [w;if read_failed then 1w else 0w]`;
+
+val STDOUT_def = Define `
+  STDOUT (output:word8 list) =
+    IO (Str (MAP (CHR o w2n) output)) stdout_fun ["putChar"] *
+    SEP_EXISTS w. W8ARRAY write_state_loc [w]`;
+
+val w2n_lt_256 =
+  w2n_lt |> INST_TYPE [``:'a``|->``:8``]
+         |> SIMP_RULE std_ss [EVAL ``dimword (:8)``]
+
+val basis_st = get_ml_prog_state;
+
+val read_spec = Q.store_thm ("read_spec",
+  `UNIT_TYPE u uv ==>
+     app (p:'ffi ffi_proj) ^(fetch_v "CharIO.read" (basis_st()))
+       [uv]
+       (STDIN input read_failed)
+       (POSTv cv. if input = "" then STDIN input T else
+                  cond (CHAR (HD input) cv) * STDIN (TL input) F)`,
+  xcf "CharIO.read" (basis_st())
+  \\ Cases_on`input = ""` \\ fs[]
+  >- (
+    fs[STDIN_def] \\ xpull
+    \\ xlet `POSTv x. STDIN "" T * cond (UNIT_TYPE () x)`
+    >- (
+      xffi
+      \\ fs[STDIN_def, EVAL ``read_state_loc``]
+      \\ `MEM "getChar" ["getChar"]` by simp[] \\ instantiate \\ xsimpl
+      \\ fs[stdin_fun_def] )
+    \\ fs[STDIN_def] \\ xpull
+    \\ xlet `POSTv x. STDIN "" T * cond (WORD (w:word8) x)`
+    >- (
+      xapp \\ xsimpl \\ fs[STDIN_def]
+      \\ fs[EVAL``read_state_loc``] \\ xsimpl)
+    \\ rw[STDIN_def] \\ xpull
+    \\ xapp \\ xsimpl \\ instantiate
+    \\ simp[w2n_lt_256] )
+  \\ fs[STDIN_def] \\ xpull
+  \\ xlet `POSTv x. IO (Str (TL input)) stdin_fun ["getChar"] *
+                    W8ARRAY read_state_loc [n2w (ORD (HD input)); 0w]`
+  >- (
+    xffi
+    \\ fs[STDIN_def, EVAL ``read_state_loc``]
+    \\ `MEM "getChar" ["getChar"]` by simp[] \\ instantiate \\ xsimpl
+    \\ fs[stdin_fun_def] )
+  \\ xlet `POSTv x. STDIN (TL input) F * cond (WORD ((n2w(ORD(HD input))):word8) x)`
+  >- (
+    xapp \\ xsimpl \\ fs[STDIN_def]
+    \\ fs[EVAL``read_state_loc``] \\ xsimpl)
+  \\ rw[STDIN_def] \\ xpull
+  \\ xapp \\ xsimpl \\ instantiate
+  \\ simp[CHR_ORD,ORD_BOUND])
+
+val read_failed_spec = Q.store_thm("read_failed_spec",
+  `UNIT_TYPE u uv ==>
+    app (p:'ffi ffi_proj) ^(fetch_v "CharIO.read_failed" (basis_st()))
+      [uv]
+      (STDIN input read_failed)
+      (POSTv bv. STDIN input read_failed * cond (BOOL read_failed bv))`,
+  xcf "CharIO.read_failed" (basis_st())
+  \\ fs[STDIN_def] \\ xpull
+  \\ xlet `POSTv x. STDIN input read_failed * cond (WORD (if read_failed then 1w else (0w:word8)) x)`
+  >- (
+    xapp
+    \\ fs[STDIN_def]
+    \\ fs[EVAL``read_state_loc``]
+    \\ xsimpl)
+  \\ fs[STDIN_def] \\ xpull
+  \\ xapp
+  \\ instantiate
+  \\ xsimpl
+  \\ rw[]);
+
+val write_spec = Q.store_thm ("write_spec",
+  `WORD c cv ==>
+     app (p:'ffi ffi_proj) ^(fetch_v "CharIO.write" (basis_st()))
+       [cv]
+       (STDOUT output)
+       (POSTv uv. cond (UNIT_TYPE () uv) * STDOUT (output ++ [c]))`,
+  xcf "CharIO.write" (basis_st())
+  \\ fs [STDOUT_def] \\ xpull
+  \\ xlet `POSTv zv. IO (Str (MAP (CHR o w2n) output)) stdout_fun ["putChar"] * W8ARRAY write_state_loc [c] *
+                     & (UNIT_TYPE () zv)`
+  THEN1
+   (xapp \\ xsimpl \\ fs [EVAL ``write_state_loc``]
+    \\ instantiate \\ xsimpl \\ EVAL_TAC \\ fs [])
+  \\ xlet `POSTv _. IO (Str (MAP (CHR o w2n) (output ++ [c]))) stdout_fun ["putChar"] * W8ARRAY write_state_loc [c]`
+  THEN1
+   (xffi
+    \\ fs [EVAL ``write_state_loc``, STDOUT_def]
+    \\ `MEM "putChar" ["putChar"]` by EVAL_TAC \\ instantiate \\ xsimpl \\ EVAL_TAC)
+  \\ xret \\ xsimpl);
+
+val _ = export_theory()
